\documentclass[letterpaper,11pt]{article}
\usepackage[T1]{fontenc}
\usepackage[utf8]{inputenc}
\usepackage[english]{babel}
\usepackage[left=1.25in,right=1.25in]{geometry}
\usepackage{lmodern}
\usepackage{amsmath}
\usepackage{amsfonts}
\usepackage{amssymb}
\usepackage{amsthm}
\usepackage{graphicx}
\usepackage{color}
\usepackage{xcolor}
\usepackage{url}
\usepackage{textcomp}
\usepackage{parskip}
\usepackage[thinc]{esdiff}

\title{Prelab 1: Simulation Using the Analog Computer}
\author{Elijah Onufrock}
\date{\today}

\begin{document}

\maketitle

Transfer function: $H(s) = \frac{Y(s)}{U(s)} = \frac{\omega^2_n}{s^2+2\zeta\omega_ns+\omega^2_n}$

(a) Differential Equation: $\diff[2]{y(t)}{t} = -2\zeta\omega_n\diff{y(t)}{t} - \omega_n^2y(t)+\omega_n^2u$
(with zero initial conditions)
(b) In normalized time:

\begin{center}
	$\diff[2]{y}{(\tau/\omega_n)} $
	$= -2\zeta\omega_n\diff{y}{(\tau/\omega_n)} - \omega_n^2y+\omega_n^2u$

	$\omega_n^2\diff[2]{y}{\tau}$
	$= -2\zeta\omega_n^2\diff{y}{\tau} - \omega_n^2y+\omega_n^2u$

	$\diff[2]{y}{\tau} = -2\zeta\diff{y}{\tau} - y+u$
\end{center}

(c) integrating: 
\begin{center}
	$\int(\diff[2]{y}{\tau}+2\zeta\diff{y}{\tau})d\tau$
	$ = \int(-y+u)d\tau$

	$\diff{y}{\tau}$
	$ = -2\zeta{y} + \int(u-y)d\tau d\tau$

	$y = \int(-2\zeta{y} + \int(u-y)d\tau)d\tau$
	
\end{center}
\end{document}
